

①

Assignment-1
Real AnalysisPratyush Raj
23/MC/110Ans. (a) given, $a \in \mathbb{R}$ and $a \cdot a = a$ Case 1) $a = 0$, as $0 \cdot 0 = 0$ hence a can be 0.Case 2) $a \neq 0$, hence $\exists b$ such that $ab = ba = 1$

(Existence of Inverse of multiplication)

$$a \cdot a = a$$

$$(a \cdot a) \cdot b = a \cdot b \quad [\text{multiplying both sides by } b]$$

$$a \cdot (a \cdot b) = 1 \quad [\text{associative law}]$$

$$a \cdot 1 = a = 1 \quad [x \cdot 1 = x, \text{ Identity}]$$

hence we conclude that $a \in \{0, 1\}$.(b) as $a, b \neq 0$ hence $ab \neq 0 \Rightarrow$ Inverse of ab exists, that is $\exists x \in \mathbb{R}$ such that

$$(ab)x = x(ab) = 1 \quad [\text{multiplicative Inverse}]$$

as multiplication over \mathbb{R} is an abelian group

$$\text{hence, } (ab)x = x(ab) \quad [\text{Commutative law}]$$

$$(ab)x = 1$$

$$\frac{1}{a} \cdot (ab)x = \frac{1}{a} \cdot 1 \quad [\text{multiplying both sides by multiplicative Inverse of } a]$$

$$\left(\frac{1}{a} \cdot a\right) \cdot b \cdot x = \frac{1}{a} \quad [\text{associative and Identity law}]$$

$$1 \cdot b \cdot x = \frac{1}{a} \Rightarrow b \cdot x = \frac{1}{a}$$

$$\text{for } (b \cdot x) \cdot \frac{1}{b} = \frac{1}{a} \cdot \frac{1}{b} \text{ (post multiply by } \frac{1}{b})$$

$$(x \cdot b) \cdot \frac{1}{b} = \frac{1}{a} \cdot \frac{1}{b} \text{ (Commutative law)}$$

$$x \cdot (b \cdot \frac{1}{b}) = \frac{1}{a} \cdot \frac{1}{b} \text{ (associative law)}$$

$$x \cdot 1 = \frac{1}{a} \cdot \frac{1}{b} \text{ (} x \cdot \frac{1}{x} = 1 \text{)}$$

$$x = \frac{1}{a} \cdot \frac{1}{b}$$

as x is inverse of ab , hence, $\frac{1}{(ab)} = \frac{1}{a} \cdot \frac{1}{b}$

Ans. To Prove $a^{m+n} = a^m \cdot a^n$, where $a \in \mathbb{R}$ and $m, n \in \mathbb{N}$

$$\begin{aligned} \text{Base Step (for } m=1 \text{); } a^{1+n} &= \underbrace{a \cdot \dots \cdot a}_{n+1 \text{ times}} \\ &= a \cdot \underbrace{a \cdot \dots \cdot a}_{n \text{ times}} = a \cdot a^n \text{ hence proved.} \end{aligned}$$

Induction Step: let $a^{m+n} = a^m \cdot a^n \quad \forall m \in \{1, 2, 3, \dots, k\}$.

$$\text{hence, } a^{k+n} = a^k \cdot a^n$$

$$a \cdot a^{k+n} = a(a^k \cdot a^n) \text{ (premultiply by } a \text{)}$$

$$a^{k+1+n} = (a \cdot a^k) \cdot a^n \text{ (associative law)}$$

$$a^{(k+1)+n} = a^{k+1} \cdot a^n$$

hence, we conclude that $T(k) \rightarrow T(k+1) \quad \forall k \in \mathbb{N}$
hence, proved.

$(a^m)^n$ from definitions of exponents, can be rewritten as
 $\underbrace{a^m \cdot a^m \cdot a^m \cdots a^m}_{n \text{ times}} = \text{①}$

from previous results $a^m \cdot a^m = a^{m+m} \quad (m=1)$

or, $\underbrace{a^m \cdot a^m}_{2 \text{ times}} = a^{2m}$

Similarly, let $\underbrace{a^m \cdot a^m \cdots a^m}_k = a^{km} \quad \forall k \in \{1, \dots, t\}$

Induction step: To check for $k = t+1$,

$$\underbrace{a^m \cdots a^m}_t = a^{tm}$$

$$a^m \cdot \underbrace{(a^m \cdots a^m)}_{t \text{ times}} = a^m \cdot a^{tm} \quad (\text{pre multiply by } a^m)$$

$$\underbrace{a^m \cdot a^m \cdots a^m}_{(t+1) \text{ times}} = a^{m+tm} \quad (\text{from previous result})$$

$$(a^m)^{t+1} = a^{m(1+t)} \quad [\text{distributive law}]$$

hence, $T(k) \rightarrow T(k+1)$ hence, $(a^m)^n = a^{mn}$
 is true for all $m, n \in \mathbb{N}$ and $a \in \mathbb{R}$.

Ans/ (a) by definition we know that ④
 $x^2 \leq y^2 \iff |x| \leq |y|$ — ①

$$|a| \geq a \text{ and } |b| \geq b \quad \forall a, b \in \mathbb{R}$$

$$|a| \cdot |b| \geq a \cdot b$$

$$2|a| \cdot |b| \geq 2 \cdot a \cdot b \quad (\text{as } 2 > 0)$$

$$(-1) \cdot 2|a| \cdot |b| \leq (-1) \cdot 2 \cdot a \cdot b \quad (\text{as } (-1) < 0)$$

$$-2|a| \cdot |b| \leq -2 \cdot a \cdot b$$

$$|a|^2 + |b|^2 - 2|a| \cdot |b| \leq |a|^2 + |b|^2 - 2 \cdot a \cdot b$$

(adding $|a|^2 + |b|^2$ in both sides)

$$(|a| - |b|)^2 \leq a^2 + b^2 - 2ab \quad (|a|^2 = a^2)$$

$$(|a| - |b|)^2 \leq (a-b)^2 \quad \left[(x-y)^2 = x^2 + y^2 - 2xy \right]$$

\hookrightarrow ②

from ① and ②

$$||a| - |b|| \leq |a - b| \quad \underline{\text{hence proved.}}$$

(b). for $a, b \in \mathbb{R}$

$$a \cdot b \leq |a| \cdot |b| \text{ — ①}$$

$$-2 \leq 0 \leq 2 \quad (\text{as } 2 = 1+1 > 0+0 > 0)$$

\hookrightarrow ③

$$-2 \cdot (a \cdot b) \leq 2|a| \cdot |b| \quad (\text{multiplying both ① \& ③})$$

$$a^2 + b^2 - 2ab \leq a^2 + b^2 + 2|a| \cdot |b| \quad (\text{adding } a^2 + b^2 \text{ both sides})$$

$$(a-b)^2 \leq |a|^2 + |b|^2 + 2|a||b| \quad (|x|^2 = x^2) \quad (5)$$

$$(a-b)^2 \leq (|a|+|b|)^2 \quad (\text{Identity } (x+y)^2 = x^2 + y^2 + 2xy)$$

$$|a-b| \leq |a|+|b|$$

$$|a-b| \leq |a|+|b| \leq |a|+|b| \quad (\text{as } |a| \geq 0$$

$$|a-b| \leq |a|+|b| \text{ hence proved.} \quad |b| \geq 0)$$

Any. let $\varepsilon > 0$, and define neighborhood of a as $V_\varepsilon(a) = (a-\varepsilon, a+\varepsilon)$.

let $x \in (a-\varepsilon, a+\varepsilon)$, $\forall \varepsilon \in \mathbb{R}$ and $\varepsilon > 0$

$$\Rightarrow a-\varepsilon < x < a+\varepsilon, \quad \forall \varepsilon > 0$$

$$\Rightarrow -\varepsilon < x-a < \varepsilon, \quad \forall \varepsilon > 0$$

$$\Rightarrow |x-a| < \varepsilon, \quad \forall \varepsilon > 0 \quad - \quad (1)$$

\nexists like let $x \neq a \Rightarrow x = a+t$, for some $t \in \mathbb{R}$, where $t \neq 0$. - (2)

substitute (2) in (1),

$$|x-a| < \varepsilon \Rightarrow |a+t-a| < \varepsilon \Rightarrow |t| < \varepsilon \quad \forall \varepsilon > 0$$

$$\text{let } \varepsilon = |t|/2 \Rightarrow |t| < |t|/2 \Rightarrow |t| < 0,$$

contradicting the definition of $|t|$ hence,

$$t=0 \Rightarrow x=a \text{ hence proved.}$$

Ans. Completeness property of \mathbb{R} : Given a non-empty subset $X \subseteq \mathbb{R}$, such that it contains atleast one $y \in X$, such that $y \geq x, \forall x \in X$ then $\text{Supremum}(X)$ exists in \mathbb{R} . [Similar definition for $\text{Infimum}(X)$ form.]

$$a) S_1 = \left\{ 1 - \frac{(-1)^n}{n} \mid n \in \mathbb{N} \right\}$$

$$\text{as } n > 0 \Rightarrow \frac{1}{n} > 0 - (1)$$

$$\text{as } n \geq 1 \Rightarrow \frac{1}{n} \leq 1 \Rightarrow -\frac{1}{n} \geq -1 - (2)$$

$$\text{as } -\frac{1}{n} \leq \frac{(-1)^n}{n} \leq \frac{1}{n} \quad [\text{as } -1 \leq (-1)^n \leq 1]$$

$$\Rightarrow -\frac{1}{n} \leq -\frac{(-1)^n}{n} \leq \frac{1}{n} - (3)$$

Combining (2) and (3)

$$-1 \leq -\frac{1}{n} \leq -\frac{(-1)^n}{n} \leq \frac{1}{n} \Rightarrow$$

$$1-1 \leq 1 - \frac{(-1)^n}{n} \leq 1 + \frac{1}{n} \quad (\text{adding } 1)$$

$$\boxed{0 \leq t_n \leq 1 + \frac{1}{n}, \forall n \in \mathbb{N}} - (4)$$

Combining (2) and (4)

$$0 \leq t_n \leq 1 + \frac{1}{n} \leq 2 \Rightarrow \boxed{0 \leq t_n \leq 2}$$

$$(b) S_2 = \left\{ \frac{1}{n} - \frac{1}{m} \mid n, m \in \mathbb{N} \right\} \quad (8)$$

$$\text{as } n \geq 1 \Rightarrow 0 < \frac{1}{n} \leq 1 \Rightarrow \frac{1}{n} - \frac{1}{m} \leq 1 - \frac{1}{m} \quad (1)$$

$$\text{Similarly } 0 < \frac{1}{m} \leq 1 \Rightarrow 0 > -\frac{1}{m} \geq -1 \quad (2)$$

Combining (1) and (2)

$$0 - \frac{1}{m} \leq \frac{1}{n} - \frac{1}{m} \leq \frac{1}{n} \leq 1 \Rightarrow -1 \leq -\frac{1}{m} \leq \frac{1}{n} - \frac{1}{m} \leq 1$$

$$\text{or } \boxed{-1 \leq \frac{1}{n} - \frac{1}{m} \leq 1} \quad \forall m, n \in \mathbb{N} \quad (3)$$

from (3) we conclude that, $\sup(S_2) \leq 1$
and $\inf(S_2) \geq -1 \quad (4)$

~~as for~~ n

$$\text{let } \sup(S_2) = 1 - \epsilon, \epsilon > 0 \Rightarrow$$

$$\frac{1}{n} - \frac{1}{m} < 1 - \epsilon, \forall n, m \in \mathbb{N}$$

$$\Rightarrow 1 - \frac{1}{m} \leq 1 - \epsilon, \forall m \in \mathbb{N}$$

$$\Rightarrow \frac{1}{m} \geq \epsilon \quad \forall m \in \mathbb{N}, \text{ contradicting the}$$

Archimedean Property hence, $\sup(S_2) \geq 1 \quad (5)$

Combining (4) and (5) $\boxed{\sup(S_2) = 1}$

$$\text{let's consider } -S_2 = \left\{ \frac{1}{m} - \frac{1}{n} \mid m, n \in \mathbb{N} \right\}$$

$$\text{from observation } S_1 = -S_2 \quad (6)$$

hence, $S_1 \subseteq \mathbb{R}$ contains lower bound as 0 and upper bound as 2, hence $\exists l$ and u such that $l, u \in \mathbb{R}$ and $\underline{l = \inf(S_1)}$ and $\underline{u = \sup(S_1)}$.

as for $n=1$, $t_1 = 1 - \frac{(-1)^1}{1} = 2$.

hence, $\sup(S_1) \geq 2$ and 2 is an upper bound hence, 2 is least upper bound i.e.

$$\boxed{\sup(S_1) = 2.}$$

let's focus on $f_{2n} = 1 - \frac{1}{2n} \leq 1$

as $\frac{1}{n} \leq 1 \Rightarrow \frac{1}{2n} \leq \frac{1}{2} \Rightarrow -\frac{1}{2n} \geq -\frac{1}{2}$

$1 - \frac{1}{2n} \geq \frac{1}{2}$ (hence $\frac{1}{2}$ is a lower bound of sequence t_n) - ⑤

also, note that $t_{n-1} = 1 + \frac{1}{2n-1} \geq 1 > \frac{1}{2}$

hence $\frac{1}{2}$ is a lower bound for all $t_i \in S_1$,

$\Rightarrow \inf(S_1) \geq \frac{1}{2}$ - ⑥

as $t_2 = 1 - \frac{1}{2} = \frac{1}{2} \Rightarrow \inf(S_1) \leq \frac{1}{2}$ - ⑦

Combining ⑥ and ⑦

$$\boxed{\inf(S_1) = \frac{1}{2}.}$$

in other words, $\sup(S_2) = \sup(-S_2)$ (9)

$$\sup(S_2) = -\inf(S_2) \quad \left\{ \sup(X) = \inf(-X) \right\}$$

$$\Rightarrow \boxed{\inf(S_2) = -\sup(S_2) = -1}$$

hence, prol.

$$(c) S_3 = \{x \in \mathbb{R} \mid x > 0\}$$

as, $\forall x \in \mathbb{R}$, $\exists n \in \mathbb{N}$ such that $n > x$,

hence S_3 does not contain an upper bound
i.e., $\sup(S_3)$ does not exist.

as $0 < x$, hence 0 is a lower bound of $S_3 \subseteq \mathbb{R}$
and $1 \in S_3$ hence S_3 is non empty $\Rightarrow S_3$ contains
a lower bound.
maximum

let $\varepsilon > 0$ be the $\inf(S_3) \Rightarrow 0 < \varepsilon \leq x$, $\forall x > 0$

let $x = 1/n$, where $n \in \mathbb{N}$

$\Rightarrow 0 < \varepsilon \leq 1/n$, $\forall n \in \mathbb{N}$, which contradicts
with Archimedean Property hence, $\inf(S_3) \leq 0$.

Also, as $0 < x$, $\forall x \in S_3 \Rightarrow \boxed{\inf(S_3) = 0}$

Ans/. let $X = \{x \in \mathbb{R} \mid x^2 < 2\}$, as $1 \in X$, and
 $x < 2$, $\forall x \in X \Rightarrow X$ contains a Supremum(X),
 $\in \mathbb{R}$, by Order Completeness Property.

let $y = \sup(X)$ ~~to~~ \mathbb{R}

(10)

Case 1) $y^2 < 2$.

Consider $y + \epsilon$, $\epsilon > 0$, let

$$(y + \epsilon)^2 < 2 \text{ if}$$

$$y^2 + 2y\epsilon + \epsilon^2 < 2 \text{ if}$$

$$2y\epsilon + \epsilon^2 < 2 - y^2 \text{ if}$$

$$2y\epsilon + \epsilon^2 < 2y\epsilon + \epsilon < 2 - y^2 \text{ if}$$

$$\epsilon < \frac{2 - y^2}{2y + 1}, \text{ we conclude that } \exists \epsilon > 0$$

such that $y < y + \epsilon$ and $(y + \epsilon)^2 < 2$, which means y^2 isn't ~~an~~ a sup can't be ^{the} supremum of set X .

Case 2). let $y^2 > 2$

Consider $y - \epsilon$, $\epsilon > 0$, let

$$(y - \epsilon)^2 > 2 \text{ if}$$

$$y^2 - 2 > -\epsilon^2 + 2y\epsilon \text{ if}$$

$$y^2 - 2 > 2y\epsilon > 2y\epsilon - \epsilon^2 \text{ if}$$

$$\epsilon < \frac{y^2 - 2}{2y}, \text{ we conclude that } \exists \epsilon > 0, \text{ such}$$

that $y - \epsilon < y$ and $(y - \epsilon)^2 > 2 \Rightarrow y^2 > 2$,

10

satisfying $y^2 > 2$, can't be the $\sup(x)$, that ¹¹
is $\exists y \in \mathbb{R}$ such that $y^2 = 2$. hmm find.

b) let \exists a rational number $\frac{p}{q}$, where $p, q \in \mathbb{Z}$
and $(\frac{p}{q})^2 = 2$.

let's choose p and q such that $\text{hcf}(p, q) = 1$

$$(\frac{p}{q})^2 = 2 \Rightarrow \frac{p^2}{q^2} = 2 \Rightarrow \frac{p^2}{q^2} \cdot q^2 = 2 \cdot q^2 \quad (\text{multiplying both sides by } q^2)$$

$$p^2 = \overset{\textcircled{1}}{2q^2} \Rightarrow 2 \mid p^2 \Rightarrow 2 \mid p \Rightarrow p \text{ is even}$$

that is $p = 2x$, for some $x \in \mathbb{Z}$.

Substitute p in equation ^①

$$(2x)^2 = 2q^2 \Rightarrow 4x^2 = 2q^2 \Rightarrow \frac{1}{2} \cdot 4x^2 = q^2$$

$$q^2 = 2x^2 \Rightarrow 2 \mid q^2 \Rightarrow 2 \mid q \Rightarrow q \text{ is divisible by } 2 \text{ that is } \underline{q = 2m}, \text{ for some } m \in \mathbb{Z}.$$

$$\text{as } 2 \mid p \text{ and } 2 \mid q \Rightarrow 2 \mid \text{hcf}(p, q) \Rightarrow$$

$2 \mid 1$, contradiction arises because, our assumption that $x^2 = 2$ where x is rational was wrong.

Ans 8. Bernoulli's Inequality: for $x \geq -1$ and $r \geq 1$, $(1+x)^r \geq 1+rx$, where $r \in \mathbb{N}$

for $r=1$. $(1+x)^1 \geq 1+x$

for $r \neq 1$, let $x = \frac{1}{3} + \epsilon$ ($\epsilon \neq 0$)

$(1+x)^{1+\epsilon} \geq 1 + \frac{1}{3}(1+\epsilon)$ if

$(1+x)(1+x)^\epsilon \geq (1+x) + \frac{1}{3}\epsilon$ if

$(1+x)^\epsilon \geq 1 + \frac{1}{3}\epsilon$ for $x \geq -1$ and $\epsilon > 0$

let $(1+x)^r \geq 1+rx$, $\forall r \in \{1, 2, \dots, k\}$

$(1+x)^k \geq 1+xk$ [as, $1+x \geq 0$]

$(1+x)(1+x)^k \geq (1+x)(1+xk)$ [premultiplying by $(1+x)$]

$(1+x)^{1+k} \geq 1+x(1+k) + x^2k \geq 1+x(1+k)$

$(1+x)^{1+k} \geq 1+x(k+1)$

hence, $T(k) \rightarrow T(k+1)$ and $T(1)$ is True,
So by Mathematical Induction, $(1+x)^r \geq 1+rx$
 $\forall r \in \mathbb{N}$.

Ans. Countable Set: A Set X is called ⁽¹³⁾ countable if $\exists f$, a bijective function from X to $Y \subseteq \mathbb{N}$.

Let R be a Countable Set, as $\mathbb{N} \subseteq \mathbb{R}$ hence, if R is countable then $f: \mathbb{R} \rightarrow \mathbb{N}$ must be bijective, let f be chosen such that,

$$x < y \iff f(x) < f(y) \quad \forall x, y \in \mathbb{R} \text{ and } x, y \in \mathbb{R}$$

$$x_1 = 0.45783... \rightarrow 1234009... \quad n_1$$

$$x_2 = 10.983... \rightarrow 8376400... \quad n_2$$

$$x_3 = 20.678... \rightarrow 983100...$$

we conclude that given any two x_1, x_2
 $\exists n_1, n_2 \in \mathbb{N}$.

we conclude that \exists exactly $(n_2 - n_1 - 1)$ terms between x_1 and x_2 , let that be

$$X = \{q_1, q_2, \dots, q_{n_2 - n_1 - 1}\}$$

$$\text{let define } y = \frac{q_1 + \dots + q_{n_2 - n_1 - 1}}{n_2 - n_1 - 1}$$

$$\text{we conclude that } f(\text{Sup}(X)) = \frac{1}{2} \{n_1 + 1, \dots, n_2 - 1\}$$

$$\text{Similarly } f[\text{Inf}(X - \circ r_2)] = n_2 - 2$$

that is $q_{n_2-n_1-2} < q_{n_2-n_1-1}$.

but $\bar{x} = \frac{q_{n_2-n_1-2} + q_{n_2-n_1-1}}{2} \in X$, don't have
it's image in \mathbb{N} , hence such mapping does not
exist.

Ans 10. Between any two real numbers x and y
 \exists a rational r , such that $x < r < y$.

Similarly, $\exists r'$ between $\sqrt{2}x$ and $\sqrt{2}y$

$$\sqrt{2}x < r' < \sqrt{2}y \Rightarrow x < \frac{r'}{\sqrt{2}} < y$$

now, $\frac{r'}{\sqrt{2}} \notin \mathbb{Q}$ [as let $\frac{r'}{\sqrt{2}} = q \in \mathbb{Q} \Rightarrow \sqrt{2} \in \mathbb{Q}$,
which is not the case]

hence, between any 2 ~~ration~~ reals there
exist an irrational number q , $x < q < y$.